\subsection{Automorphisms}

\begin{definition}
	Let $G$ be a group. For $a \in G$ define 

	\begin{equation}
		\iota_a: \begin{cases}
			G \to G\\
			x \mapsto axa^{-1}
		\end{cases}
	\end{equation}

	Further

	\begin{equation}
		\Inn(G) := \cbr[0]{\iota_a : a \in G}
	\end{equation}
\end{definition}

\vspace{2mm}

\begin{lemma}
	We have $\iota_a \in \Aut(G)$ for any $a \in G$. Furthermore $\Inn(G) \unlhd \Aut(G)$.
\end{lemma}

\begin{proof}
	$\iota_a \in \Aut(G)$ and $\Inn(G) \leq \Aut(G)$ is obvious. Let $\iota_a \in \Inn(G)$ and $\varphi \in \Aut(G)$. Then for $x \in G$ 

	\begin{equation*}
		\varphi\iota_a\varphi^{-1}(x) = \varphi(a \varphi^{-1}(x)a^{-1}) = \varphi(a)x\varphi(a)^{-1}
	\end{equation*}

	\noindent so $\varphi \iota_{a} \varphi^{-1} = \iota_{\varphi(a)} \in \Inn(G)$.
\end{proof}

\vspace{2mm}

\begin{lemma}
	The mapping 

	\begin{equation}
		\iota: \begin{cases}
			G \to \Aut(G)\\
			a \mapsto \iota_a
		\end{cases}
	\end{equation}

	\noindent is a homomorphisms. Furthermore $\ker(\iota) = Z(G)$.
\end{lemma}

\begin{proof}
	That $\iota \in \Hom(G,\Aut(G))$ is obvious. For $a \in \ker(\iota)$ we must have that $\iota_a = \id$, so $axa^{-1} = x$ for any $x \in G$. Hence $a \in Z(G)$. The converse is trivial.
\end{proof}

Thus by the first isomorphism theorem we have 

\begin{equation*}
	G/Z(G) \cong \Inn(G)
\end{equation*}

\begin{proposition}
	Let $G$ be a group and assume $G/Z(G)$ is cyclic. Then $G$ is abelian.
\end{proposition}

\begin{proof}
	Since $G/Z(G)$ is cyclic we have $G/Z(G) = \langle g Z(G) \rangle$ for some $g \in G$. Furthermore, each element of $G/Z(G)$ has the form $(gZ(G))^k = g^kZ(G)$ since $Z(G) \unlhd G$ and $k \in \mathbb{Z}$. Let $x,y \in G$. Since $G/Z(G)$ provides a partition of $G$ we have $x = g^m z$ and $y = g^nz'$ for some $m,n \in \mathbb{Z}$, $z,z' \in Z(G)$. Therefore 

	\begin{equation*}
		xy = g^mz g^n z' = g^m g^n zz' = g^{m + n}zz' = g^n g^m z z' = g^n g^m z'z = g^n z' g^m z = yx
	\end{equation*}

	\noindent since center elements commute with every group element.
\end{proof}
